proof/spec/Rq.ec
@@ -36,25 +36,15 @@ op (&-) (p : poly) : poly =  map Zq.([-]) p.
 
 (* Compression/decompression of polys *)
 
-op compress_poly(d : int, p : poly) : int Array256.t =  map (compress d) p.
+op compress_poly(d : int, p : poly) : int Array256.t =  map (Compress d) p.
 
-op decompress_poly(d : int, p : int Array256.t) : poly =  map (decompress d) p.
+op decompress_poly(d : int, p : int Array256.t) : poly =  map (Decompress d) p.
 
 
 (**************************************************)
 (**************************************************)
 
-(* The NTT operation over ring elements 
-
-We give here the mathematical specification of the NTT in
-a way that roughly matches what is described in the spec.
-
-Then we will have an NTT.ec file where we prove that 1) the imperative
-specs are equivalent to these operators and 2) that these operators have
-the properties we require to show that MLKEM is correct up to some
-decryption failure bound.
-
-*)
+(* The NTT operation over ring elements *)
 
 require (****) Bigalg.
 clone import Bigalg.BigComRing as BigDom with
@@ -115,3 +105,143 @@ op basemul(a b : poly) :  poly = Array256.init (fun i =>
   else let ii = i %/ 2 in 
   (cmplx_mul (a.[2*ii],a.[2*ii+1]) (b.[2*ii],b.[2*ii+1]) (ZqRing.exp zroot ((2 * br ii + 1)))).`2).
 
+
+(* ------------------------------------------------------------------ *)
+(* Algebraic poly-ring bridge: poly = coeff Array256.t viewed as the
+   PolyReduce ring Zq[X]/(X^256+1) (AlgR), with poly2polyr/polyr2poly
+   conversions and the lift lemmas. Relocated here (was in Correctness768)
+   so the algebraic Matrix clone in VecMat can sit at the top of the
+   type hierarchy, mirroring formosa-mldsa. *)
+(* ------------------------------------------------------------------ *)
+
+require import PolyReduce. 
+clone import PolyReduce as RqTheory with
+   op n <- 256,
+   type coeff <- coeff,
+   op Coeff.(+) <- Zq.(+),
+   op Coeff.( *) <- Zq.( *),
+   op Coeff.zeror <- Zq.zero,
+   op Coeff.oner <- Zq.one,
+   op Coeff.([-]) <- Zq.([-]),
+   op Coeff.invr <- Zq.inv,
+   pred Coeff.unit <- Zq.unit
+   rename "polyXnD1" as "AlgR"
+   rename "poly" as "basepoly"
+   proof Coeff.addrA by apply ZqRing.addrA
+   proof Coeff.addrC by apply ZqRing.addrC
+   proof Coeff.add0r by apply ZqRing.add0r 
+   proof Coeff.addNr by apply ZqRing.addNr 
+   proof Coeff.oner_neq0 by apply ZqRing.oner_neq0
+   proof Coeff.mulrA by apply ZqRing.mulrA
+   proof Coeff.mulrC by apply ZqRing.mulrC 
+   proof Coeff.mul1r by apply ZqRing.mul1r 
+   proof Coeff.mulrDl by apply ZqRing.mulrDl 
+   proof Coeff.mulVr by apply ZqRing.mulVr
+   proof Coeff.unitP by apply ZqRing.unitP 
+   proof Coeff.unitout by apply ZqRing.unitout
+   proof gt0_n by auto.
+   (* proof *. fix me *)
+
+op poly2polyr(p : poly) : AlgR = pi (oget (BasePoly.to_basepoly 
+                              (fun i => if 0<=i<256 then p.[i] else Zq.zero))).
+op polyr2poly(p : AlgR) : poly = Array256.init (fun i => p.[i]).
+
+lemma poly2polyrP i p :  0<=i<256 => (poly2polyr p).[i] = p.[i].
+move => ib.
+have H := (BasePoly.to_basepolyT (fun (i0 : int) => if 0 <= i0 && i0 < 256 then p.[i0] else Zq.zero) _).
+ split; first smt(). 
+ by exists 256; smt().
+rewrite /poly2polyr /"_.[_]".
+rewrite piK. 
++ rewrite reducedP /=.
+  apply BasePoly.deg_leP => //. 
+  move=> j Hj /=. 
+  move: H; pose P:= BasePoly.to_basepoly _.
+  have: P=P by done.
+  by move: {1}P => [|pol] /#.
+move: H; pose P:= BasePoly.to_basepoly _.
+have: P=P by done.
+by move: {1}P => [|pol] /#.
+qed.
+
+lemma polyr2polyP i p :  0<=i<256 => (polyr2poly p).[i] = p.[i].
+move => ib;rewrite /polyr2poly /"_.[_]" initiE //=.
+qed.
+
+
+lemma polyr2polyK : cancel poly2polyr polyr2poly.
+rewrite /cancel => x; apply Array256.tP => i ib.
+by rewrite polyr2polyP // poly2polyrP //=.
+qed.
+
+lemma poly2polyrK : cancel polyr2poly poly2polyr.
+rewrite /cancel => x;  apply AlgR_eqP => i ib.
+by rewrite poly2polyrP // polyr2polyP //=.
+qed.
+
+lemma add_lift a b : a &+ b = polyr2poly (poly2polyr a + poly2polyr b). 
+apply Array256.tP => i ib.
+rewrite polyr2polyP // rcoeffD !poly2polyrP //.
+by rewrite /(&+) /= map2E /= initiE //=.
+qed.
+
+lemma sub_lift a : (&-) a = polyr2poly (- poly2polyr a). 
+apply Array256.tP => i ib.
+rewrite polyr2polyP // -rcoeffN !poly2polyrP //.
+by rewrite /(&-) /= mapE /= initiE //=.
+qed.
+
+lemma mul_lift a b : a &* b = polyr2poly (poly2polyr a * poly2polyr b). 
+apply Array256.tP => i ib.
+rewrite polyr2polyP // rcoeffM //. 
+rewrite /(&*) /= /BasePoly.BigCf.BCA.big filter_predT /range /= initiE  //= foldr_map /=.
+have : forall x, x \in (iota_ 0 256) => 0 <= x < 256 by smt(mem_iota).
+elim (iota_ 0 256).
++ by auto.
+move => x l H H1 /=.
+case (0 <= i - x).
+ + move => * /=.
+   rewrite (H _) /=.
+    by move=> y Hy; apply H1 => /= /#.
+   ring.
+   have -> : (poly2polyr b).[256 + i - x] = Zq.zero by smt(lt0_rcoeff gered_rcoeff).
+   rewrite poly2polyrP; 1: by smt(mem_head). 
+   rewrite poly2polyrP; 1: by smt().
+   by ring.
+move => * /=.
+rewrite (H _) /=. 
+ by move=> y Hy; apply H1 => /= /#.
+ring.
+rewrite poly2polyrP; 1: smt().
+rewrite poly2polyrP; 1: by smt(mem_head). 
+   have -> : (poly2polyr b).[i - x] = Zq.zero by smt(lt0_rcoeff gered_rcoeff).
+   have -> : 256 + (i - x) = 256 + i - x by smt().
+   by ring.
+qed.
+
+lemma zero_lift : zero = polyr2poly zeroXnD1. 
+apply Array256.tP => i ib.
+by rewrite polyr2polyP // /zero /create initiE //= rcoeff0.
+qed.
+
+lemma one_lift : one = polyr2poly oneXnD1. 
+apply Array256.tP => i ib.
+rewrite polyr2polyP // /one /zero /create.
+case (i = 0).
+move => *;rewrite set_eqiE //;1: 
+  by smt(BasePoly.lc1 creprK piK reduced1 BasePoly.deg1).
+by move => *; rewrite set_neqiE // initiE //=;
+ smt(BasePoly.gedeg_coeff creprK piK reduced1 BasePoly.deg1).
+qed.
+
+lemma polyr2poly_inj : injective polyr2poly.
+by apply (can_inj _ poly2polyr); apply poly2polyrK.
+qed.
+
+lemma poly2polyr_inj : injective poly2polyr.
+by apply (can_inj _ polyr2poly); apply polyr2polyK.
+qed.
+
+(* Fix me PY: We currently don't care about inverting polynomials *)
+op unit(p : poly) = exists q, q &* p = one.
+op invr(p : poly) = choiceb (fun q => q &* p = one) p.
